Code/Syntax/StrongNormalization/BetaReductionSN.v
@@ -1,216 +1,13 @@
+Require Import Prelude.Funext.
 Require Import Prelude.Basics.
-Require Import Prelude.Wellfounded.
+Require Import Prelude.WellfoundedRelation.
+Require Import Prelude.TransitiveClosure.
 Require Import Syntax.Signature.
 Require Import Syntax.Signature.SubstitutionLemmas.
+Require Import Syntax.Signature.RewriteLemmas.
 Require Import Syntax.StrongNormalization.SN.
+Require Import Syntax.StrongNormalization.BetaNormalForm.
 Require Import Coq.Program.Equality.
-
-(** * Strongly normalizing terms *)
-Definition term_isSN
-           {B : Type}
-           {F : Type}
-           {ar : F -> ty B}
-           {C : con B}
-           {A : ty B}
-           (t : tm ar C A)
-  : Prop
-  := isWf (fun (t1 t2 : tm ar C _) => betaRed t1 t2) t.
-
-(** Base terms and variables are strongly normalizing *)
-Lemma is_BaseTm_transport
-      {B : Type}
-      {F : Type}
-      {ar : F -> ty B}
-      {C : con B}
-      {A1 A2 : ty B}
-      (p : A1 = A2)
-      (t : tm ar C A1)
-  : is_BaseTm (transport _ p t) -> is_BaseTm t.
-Proof.
-  subst.
-  exact (fun x => x).
-Qed.
-
-Lemma baseTm_is_nf_help
-      {B : Type}
-      {F : Type}
-      {ar : F -> ty B}
-      {C : con B}
-      {A : ty B}
-      (t1 t2 : tm ar C A)
-      (f : F)
-      (p1 : ar f = A)
-      (p2 : transport (tm ar C) p1 (BaseTm f) = t1)
-  : betaRed t1 t2 -> False.
-Proof.
-  intro q.
-  revert p2.
-  revert p1.
-  revert f.
-  induction q ; intros f' p1 p2.
-  - apply (IHq1 f' p1 p2).
-  - subst.
-    discriminate p2.
-  - subst.
-    discriminate p2.
-  - apply (is_BaseTm_transport (eq_sym p1) (λ f1)).
-    rewrite <- p2.
-    rewrite transport_sym_p.
-    simpl.
-    auto.
-  - subst.
-    cbn in *.
-    discriminate p2.
-Qed.
-
-Lemma baseTm_is_nf
-      {B : Type}
-      {F : Type}
-      {ar : F -> ty B}
-      {C : con B}
-      (f : F)
-      (t : tm ar C (ar f))
-  : betaRed (BaseTm f) t -> False.
-Proof.
-  exact (baseTm_is_nf_help (BaseTm f) t f eq_refl eq_refl).
-Qed.
-
-Proposition baseTm_is_SN
-            {B : Type}
-            {F : Type}
-            {ar : F -> ty B}
-            {C : con B}
-            (f : F)
-  : @term_isSN _ _ ar C _ (BaseTm f).
-Proof.
-  unfold term_isSN.
-  apply acc.
-  intros ? p.
-  contradiction (baseTm_is_nf f _ p).
-Qed.
-
-Lemma var_is_nf
-      {B : Type}
-      {F : Type}
-      {ar : F -> ty B}
-      {C : con B}
-      {A : ty B}
-      (v : var C A)
-      (t : tm ar C A)
-  : betaRed (TmVar v) t -> False.
-Proof.
-  intro p.
-  dependent induction p.
-  apply (IHp1 v).
-  reflexivity.
-Qed.
-
-Proposition var_is_SN
-            {B : Type}
-            {F : Type}
-            {ar : F -> ty B}
-            {C : con B}
-            {A : ty B}
-            (v : var C A)
-  : @term_isSN _ _ ar _ _ (TmVar v).
-Proof.
-  apply acc.
-  intros ? q.
-  contradiction (var_is_nf v _ q).
-Qed.
-
-(** Closed under weakening *)
-Definition betaRed_wkTm
-           {B : Type}
-           {F : Type}
-           {ar : F -> ty B}
-           {C1 C2 : con B}
-           {w : wk C1 C2}
-           {A : ty B}
-           {t2 : tm ar C2 A}
-           {t1 : tm ar C1 A}
-           (r : betaRed (wkTm t2 w) t1)
-  : { t' : tm ar C2 A | t1 = wkTm t' w }.
-Proof.
-  (*
-  revert r.
-  revert t1.
-  revert w.
-  revert C1.
-  induction t2 ; simpl in * ; intros C1 w t1 r.
-  - contradiction (@baseTm_is_nf B F ar C1 f _ r).
-  - admit.
-  - admit.
-  - specialize (IHt2_1 _ w).
-    specialize (IHt2_2 _ w).
-
-      
-  dependent induction r.
-  - specialize (IHr1 _ w t2 eq_refl).
-    destruct IHr1 as [ t1' Ht1'].
-    exact (IHr2 _ w t1' Ht1').
-  - specialize (IHr _ w).
-    admit.
-  - specialize (IHr _ w).
-    admit.
-  - admit.
-  - admit.
-   *)
-Admitted.
-
-(*
-Proposition betaRed_wkTm_from_red
-            {B : Type}
-            {F : Type}
-            {ar : F -> ty B}
-            {C1 C2 : con B}
-            (w : wk C1 C2)
-            {A : ty B}
-            {t1 : tm ar C1 A}
-            {t2 : tm ar C2 A}
-            (r : betaRed (wkTm t2 w) t1)
-  : betaRed t2 (betaRed_wkTm r).
-Proof.
-Admitted.
-
-Proposition betaRed_wkTm_to_red
-            {B : Type}
-            {F : Type}
-            {ar : F -> ty B}
-            {C1 C2 : con B}
-            (w : wk C1 C2)
-            {A : ty B}
-            {t1 : tm ar C1 A}
-            {t2 : tm ar C2 A}
-            (r : betaRed (wkTm t2 w) t1)
-  : betaRed (wkTm (betaRed_wkTm r) w) t1.
-Proof.
-Admitted.
- *)
-
-Proposition wkTm_isSN
-            {B : Type}
-            {F : Type}
-            {ar : F -> ty B}
-            {C1 C2 : con B}
-            (w : wk C1 C2)
-            {A : ty B}
-            (t : tm ar C2 A)
-            (p : term_isSN t)
-  : term_isSN (wkTm t w).
-Proof.
-  induction p as [t Ht IHt].
-  apply acc.
-  intros y r.
-  (*
-  pose (t' := betaRed_wkTm r).
-  destruct t' as [t' Ht'].
-  subst.
-  apply IHt.
-   *)
-Admitted.
-
-(** * Logical relations *)
 
 (** On terms *)
 Fixpoint logical_SN
@@ -221,7 +18,7 @@ Fixpoint logical_SN
          {A : ty B}
   : tm ar C A -> Prop
   := match A with
-     | Base b => term_isSN
+     | Base b => term_is_beta_SN
      | A1 ⟶ A2 =>
        fun f =>
          forall (C2 : con B)
@@ -243,7 +40,8 @@ Proposition wk_logical_SN
   : logical_SN (wkTm t w).
 Proof.
   destruct A.
-  - apply wkTm_isSN.
+  - simpl in *.
+    apply wkTm_is_beta_SN.
     exact Ht.
   - intros C w' t' Ht'.
     rewrite wkTm_comp.
@@ -284,7 +82,7 @@ Proposition Extend_logical_SN
             (t : tm ar C1 A)
             (p : logical_SN_sub s)
             (q : logical_SN t)
-  : logical_SN_sub (s & t).
+  : logical_SN_sub (s && t).
 Proof.
   intros A' v.
   dependent induction v ; simpl ; cbn.
@@ -300,13 +98,13 @@ Proposition Extend_logical_SN_pr1
             {s : sub ar C1 C2}
             {A : ty B}
             (t : tm ar C1 A)
-            (p : logical_SN_sub (s & t))
+            (p : logical_SN_sub (s && t))
   : logical_SN_sub s.
 Proof.
   intros A' v.
   assert (subVar v s
           =
-          subTm (TmVar (wkVar v (dropId C2 _))) (s & t)).
+          subTm (TmVar (wkVar v (dropId C2 _))) (s && t)).
   {
     rewrite wkVar_is_subVar.
     symmetry.
@@ -336,73 +134,28 @@ Proposition Extend_logical_SN_pr2
             {s : sub ar C1 C2}
             {A : ty B}
             (t : tm ar C1 A)
-            (p : logical_SN_sub (s & t))
+            (p : logical_SN_sub (s && t))
   : logical_SN t.
 Proof.
   exact (p A Vz).
 Qed.
 
 (** * Neutral terms *)
+
+(** Our goal is to show that all neutral terms satisfy the logical relation *)
 Inductive is_neutral
           {B : Type}
           {F : Type}
           {ar : F -> ty B}
           {C : con B}
-  : forall {A : ty B}, tm ar C A -> Prop
+  : forall {A : ty B}, tm ar C A -> Type
   :=
 | BaseTm_is_neutral : forall (f : F), is_neutral (BaseTm f)
 | Var_is_neutral : forall {A : ty B} (v : var C A), is_neutral (TmVar v)
 | App_is_neutral : forall {A1 A2 : ty B} (f : tm ar C (A1 ⟶ A2)) (t : tm ar C A1),
-    is_neutral f -> term_isSN t -> is_neutral (f · t).
+    is_neutral f -> term_is_beta_SN t -> is_neutral (f · t).
 
-Lemma beta_red_term_isSN
-      {B : Type}
-      {F : Type}
-      {ar : F -> ty B}
-      {C : con B}
-      {A : ty B}
-      {t1 t2 : tm ar C A}
-      (r : betaRed t1 t2)
-      (Ht1 : term_isSN t1)
-  : term_isSN t2.
-Proof.
-  revert r.
-  revert t2.
-  induction Ht1 as [t1 Ht1 IHt1].
-  intros t2 r.
-  apply acc.
-  intros t' r'.
-  exact (IHt1 t2 r t' r').
-Qed.
-
-Lemma beta_red_neutral
-      {B : Type}
-      {F : Type}
-      {ar : F -> ty B}
-      {C : con B}
-      {A : ty B}
-      {t1 t2 : tm ar C A}
-      (r : betaRed t1 t2)
-      (Ht1 : is_neutral t1)
-  : is_neutral t2.
-Proof.
-  induction r.
-  - apply IHr2.
-    apply IHr1.
-    exact Ht1.
-  - dependent destruction Ht1.
-    constructor.
-    + apply IHr ; assumption.
-    + assumption.
-  - dependent destruction Ht1.
-    constructor.
-    + assumption.
-    + exact (beta_red_term_isSN r H).
-  - inversion Ht1.
-  - dependent destruction Ht1.
-    inversion Ht1.
-Qed.
-
+(** Neutral terms are closed under weakening *)
 Lemma wk_neutral
       {B : Type}
       {F : Type}
@@ -423,10 +176,82 @@ Proof.
     constructor.
     + apply IHt1.
       assumption.
-    + apply wkTm_isSN.
-      exact H.
+    + apply wkTm_is_beta_SN.
+      exact t0.
 Qed.
 
+
+(** * Properties of the logical relation *)
+
+(** We prove two properties of logical relations, namely that neutral terms satisfy it and that each element that satisfies the relation, is strongly normalizing. We do that by mutual induction. *)
+
+(** Neutral terms reduce to neutral terms *)
+Lemma neutral_beta
+      {B : Type}
+      {F : Type}
+      {ar : F -> ty B}
+      {C : con B}
+      {A : ty B}
+      {t t' : tm ar C A}
+      (Ht : is_neutral t)
+      (r : t ~>β t')
+  : is_neutral t'.
+Proof.
+  induction r.
+  - dependent destruction Ht.
+    apply App_is_neutral.
+    + apply IHr.
+      exact Ht.
+    + exact t0.
+  - dependent destruction Ht.
+    apply App_is_neutral.
+    + exact Ht.
+    + clear IHr.
+      revert r.
+      revert x2.
+      induction t0 as [x1 Hx1 IHx1].
+      intros x2 r.
+      apply single_step_SN.
+      intros t' Ht'.
+      exact (IHx1 x2 (TStep r) t' Ht').
+  - inversion Ht.
+  - induction r.
+    dependent destruction Ht.
+    inversion Ht.
+Qed.
+
+(** If we apply a strongly normalizing neutral term to a strongly normalizing term, then we get another strongly normalizing term *)
+Lemma neutral_beta_SN
+      {B : Type}
+      {F : Type}
+      {ar : F -> ty B}
+      {C : con B}
+      {A1 A2 : ty B}
+      (f : tm ar C (A1 ⟶ A2))
+      (Hf1 : is_neutral f)
+      (Hf2 : term_is_beta_SN f)
+      (t : tm ar C A1)
+      (Ht : term_is_beta_SN t)
+  : term_is_beta_SN (f · t).
+Proof.
+  revert Ht.
+  revert t.
+  induction Hf2 as [f2 Hf2 IHf2].
+  intros t Ht.
+  induction Ht as [t Ht IHt].
+  apply single_step_SN.
+  intros t' r.
+  dependent destruction r.
+  - pose (X := neutral_beta Hf1 r).
+    specialize (IHf2 f0 (TStep r) X).
+    apply IHf2.
+    apply acc ; assumption.
+  - exact (IHt x2 (TStep r)).
+  - dependent destruction b.
+    inversion Hf1.
+Qed.
+
+(** Neutral terms satisfy the logical relation and terms that satisfy the logical relation are strongly normalizing *)
 Definition map_tm_logical_SN
            {B : Type}
            {F : Type}
@@ -436,32 +261,6 @@ Definition map_tm_logical_SN
            (f : tm ar C (A1 ⟶ A2))
   : tm ar (A1 ,, C) A2
   := wkTm f (Drop _ (idWk C)) · TmVar Vz.
-
-Definition BetaRed_Wk
-           {B F : Type}
-           {ar : F -> ty B}
-           {C1 C2 : con B}
-           {A : ty B}
-           {t1 t2 : tm ar C2 A}
-           (w : wk C1 C2)
-           (p : betaRed t1 t2)
-  : betaRed (wkTm t1 w) (wkTm t2 w).
-Proof.
-  revert w.
-  revert C1.
-  induction p ; intros C1 w ; simpl.
-  - exact (BetaTrans (IHp1 C1 w) (IHp2 C1 w)).
-  - exact (BetaRew_App_l _ (IHp C1 w)).
-  - exact (BetaRew_App_r _ (IHp C1 w)).
-  - exact (BetaRew_Lam (IHp _ (Keep A1 w))).
-  - simpl.
-    rewrite !wkTm_is_subTm.
-    rewrite subTm_comp.
-    unfold beta_sub.
-    rewrite <- beta_sub_help.
-    rewrite <- subTm_comp.
-    apply BetaBeta.
-Qed.
 
 Lemma Rew_map_tm_logical_SN
       {B : Type}
@@ -474,54 +273,11 @@ Lemma Rew_map_tm_logical_SN
   : betaRed (map_tm_logical_SN f1) (map_tm_logical_SN f2).
 Proof.
   unfold map_tm_logical_SN.
-  apply BetaRew_App_l.
+  apply beta_App_l.
   apply BetaRed_Wk.
   exact p.
 Qed.
 
-Lemma neutral_SN
-      {B : Type}
-      {F : Type}
-      {ar : F -> ty B}
-      {C : con B}
-      {A1 A2 : ty B}
-      (f : tm ar C (A1 ⟶ A2))
-      (Hf1 : is_neutral f)
-      (Hf2 : term_isSN f)
-      (t : tm ar C A1)
-      (Ht : term_isSN t)
-  : term_isSN (f · t).
-Proof.
-  revert Hf1 Hf2.
-  revert f.
-  induction Ht as [t Ht IHt].
-  intros f Hf1 Hf2.
-  induction Hf2 as [f Hf2 IHf].
-  apply acc.
-  intros y r.
-  dependent destruction r.
-  - (*assert (f' : tm ar C (A1 ⟶ A)) by admit.
-    assert (t' : tm ar C A1) by admit.
-    assert (p : t3 = f' · t') by admit.
-    assert (H : betaRed t t' + betaRed t t') by admit.
-    subst.
-    destruct H.
-    + apply IHt.
-      apply (IHf f').
-     *)
-    admit.
-  - apply (IHf f2 r).
-    exact (beta_red_neutral r Hf1).
-  - apply (IHt x2 r).
-    + exact Hf1.
-    + apply acc.
-      exact Hf2.
-  - inversion Hf1.
-Admitted.
-
-(** * Properties of the logical relation *)
-
-(** We prove two properties of logical relations, namely that neutral terms satisfy it and that each element that satisfies the relation, is strongly normalizing. We do that by mutual induction. *)
 Lemma neutral_is_logical_SN_and_logical_SN_to_SN
       {B : Type}
       {F : Type}
@@ -531,7 +287,7 @@ Lemma neutral_is_logical_SN_and_logical_SN_to_SN
            (t : tm ar C A),
     (is_neutral t -> logical_SN t)
     /\
-    (logical_SN t -> term_isSN t).
+    (logical_SN t -> term_is_beta_SN t).
 Proof.      
   induction A as [ b | A1 IHA1 A2 IHA2 ].
   - simpl.
@@ -540,7 +296,7 @@ Proof.
     + induction p.
       * apply baseTm_is_SN.
       * apply var_is_SN.
-      * apply neutral_SN ; assumption.
+      * apply neutral_beta_SN ; assumption.
     + assumption.
   - simpl.
     intros C t.
@@ -585,7 +341,7 @@ Proposition logical_SN_to_SN
   : forall {C : con B}
            {t : tm ar C A}
            (p : logical_SN t),
-    term_isSN t.
+    term_is_beta_SN t.
 Proof.
   intros C t p.
   apply (neutral_is_logical_SN_and_logical_SN_to_SN t).
@@ -644,8 +400,9 @@ Inductive repeat_app
   : ty B -> ty B -> Type
   :=
   | empty : forall (A : ty B), repeat_app ar C A A
-  | add_term : forall (A1 A2 A3 : ty B),
-      tm ar C A2
+  | add_term : forall (A1 A2 A3 : ty B)
+                      (t : tm ar C A2),
+      logical_SN t
       -> repeat_app ar C A1 (A2 ⟶ A3)
       -> repeat_app ar C A1 A3.
 
@@ -662,8 +419,8 @@ Fixpoint sem
          (ps : repeat_app ar C A1 A2)
   : tm ar C A1 -> tm ar C A2
   := match ps with
-     | empty => fun t => t
-     | add_term t qs => fun f => sem qs f · t
+     | empty => fun f => f
+     | add_term t _ qs => fun f => sem qs f · t
      end.
 
 (** Closure under weakening *)
@@ -678,7 +435,7 @@ Fixpoint wk_repeat_app
   : repeat_app ar C1 A1 A2
   := match ps with
      | empty => empty
-     | add_term t qs => add_term (wkTm t w) (wk_repeat_app qs w)
+     | add_term t Ht qs => add_term (wkTm t w) (wk_logical_SN w _ Ht) (wk_repeat_app qs w)
      end.
 
 Proposition sem_wk_repeat_app
@@ -692,7 +449,7 @@ Proposition sem_wk_repeat_app
             (t : tm ar C2 A1)
   : sem (wk_repeat_app ps w) (wkTm t w) = wkTm (sem ps t) w.
 Proof.
-  induction ps as [ | ? ? ? t' qs IHqs ].
+  induction ps as [ | ? ? ? t' ? qs IHqs ].
   - reflexivity.
   - simpl.
     rewrite IHqs.
@@ -710,7 +467,7 @@ Lemma logical_SN_beta_help
       (t : tm ar C A1)
       (Hsub : logical_SN (subTm f (beta_sub t)))
       (Hf : logical_SN f)
-      (Ht : term_isSN t)
+      (Ht : logical_SN t)
       (ps : repeat_app ar C A2 A3)
   : logical_SN (sem ps (λ f · t)).
 Proof.
@@ -720,16 +477,29 @@ Proof.
   revert C.
   induction A3 as [ b | A31 IHA31 A32 IHA32 ] ; intros C A1 A2 t f ps Ht Hf Hsub.
   - simpl.
+    assert (term_is_beta_SN (sem ps (subTm f (beta_sub t)))).
+    {
+      apply logical_SN_to_SN.
+      (* make a separate lemma *)
+      induction ps.
+      - exact Hsub.
+      - simpl.
+        pose (IHps f Hf Hsub _ (idWk _) t0 l : logical_SN _).
+        simpl in l0.
+        rewrite wkTm_id in l0.
+        exact l0.
+    }
+
     admit.
   - intros ? w t' Ht'.
     specialize (IHA32
                   _ _ _
                   (wkTm t w) (wkTm f (Keep A1 w))
-                  (add_term t' (wk_repeat_app ps w))).
+                  (add_term t' Ht' (wk_repeat_app ps w))).
     simpl in IHA32.
     rewrite <- sem_wk_repeat_app.
     apply IHA32.
-    + apply wkTm_isSN.
+    + apply wk_logical_SN.
       exact Ht.
     + apply wk_logical_SN.
       exact Hf.
@@ -761,7 +531,7 @@ Lemma logical_SN_beta
       (t : tm ar C A1)
       (Hsub : logical_SN (subTm f (beta_sub t)))
       (Hf : logical_SN f)
-      (Ht : term_isSN t)
+      (Ht : logical_SN t)
   : logical_SN (λ f · t).
 Proof.
   exact (logical_SN_beta_help f t Hsub Hf Ht empty).
@@ -832,8 +602,7 @@ Proof.
         apply wk_logical_SN.
         apply p.
       * apply var_is_logical_SN.
-    + apply logical_SN_to_SN.
-      exact Ht'.
+    + exact Ht'.
   - specialize (IHt2 _ s p).
     pose (IHt1 _ s p _ (idWk _) _ IHt2).
     rewrite wkTm_id in l.
