Code/Syntax/Signature/RewriteLemmas.v
@@ -1,0 +1,409 @@
+Require Import Prelude.Funext.
+Require Import Prelude.Basics.
+Require Import Syntax.Signature.
+Require Import Syntax.Signature.SubstitutionLemmas.
+Require Import Coq.Program.Equality.
+
+(** * Lemmas on the rewriting relation *)
+
+(** ** Beta reduction is reflected under weakening *)
+Lemma is_BaseTm_wkTm
+      {B : Type}
+      {F : Type}
+      {ar : F -> ty B}
+      {C1 C2 : con B}
+      (w : wk C1 C2)
+      {A : ty B}
+      {t : tm ar C2 A}
+      (Ht : is_BaseTm t)
+  : is_BaseTm (wkTm t w).
+Proof.
+  induction t ; try contradiction.
+  apply I.
+Qed.
+
+Definition wWeakened
+           {B : Type}
+           {F : Type}
+           {ar : F -> ty B}
+           {C1 C2 : con B}
+           (w : wk C1 C2)
+           {A : ty B}
+           (t : tm ar C1 A)
+  : Type
+  := { t' : tm ar C2 A | wkTm t' w = t  }.
+
+Definition term_of
+           {B : Type}
+           {F : Type}
+           {ar : F -> ty B}
+           {C1 C2 : con B}
+           {w : wk C1 C2}
+           {A : ty B}
+           {t : tm ar C1 A}
+           (p : wWeakened w t)
+  : tm ar C2 A.
+Proof.
+  destruct p as [x e].
+  exact x.
+Defined.
+
+Definition term_of_eq
+           {B : Type}
+           {F : Type}
+           {ar : F -> ty B}
+           {C1 C2 : con B}
+           {w : wk C1 C2}
+           {A : ty B}
+           {t : tm ar C1 A}
+           (p : wWeakened w t)
+  : wkTm (term_of p) w = t.
+Proof.
+  destruct p as [x e].
+  exact e.
+Defined.
+
+Definition wkTm_red_lam_help
+           {B : Type}
+           {F : Type}
+           {ar : F -> ty B}
+           {C1 C2 : con B}
+           (w : wk C1 C2)
+           {A1 A2 A' : ty B}
+           (t : tm ar C2 A')
+           (f : tm ar (A1 ,, C1) A2)
+           (p : A' = (A1 ⟶ A2))
+           (q : wkTm (transport _ p t) w = λ f)
+  : { t' : tm ar (A1 ,, C2) A2 | transport _ p t = λ t' }.
+Proof.
+  destruct t ; try (subst ; simpl in * ; discriminate).
+  - enough (is_BaseTm (λ f)) by contradiction.
+    rewrite <- q.
+    apply is_BaseTm_wkTm.
+    apply transport_BaseTm.
+    apply I.
+  - dependent destruction p ; simpl.
+    exists t.
+    reflexivity.
+Qed.
+
+Definition wkTm_red_lam
+           {B : Type}
+           {F : Type}
+           {ar : F -> ty B}
+           {C1 C2 : con B}
+           (w : wk C1 C2)
+           {A1 A2 : ty B}
+           (t : tm ar C2 (A1 ⟶ A2))
+           (f : tm ar (A1 ,, C1) A2)
+           (q : wkTm t w = λ f)
+  : { t' : tm ar (A1 ,, C2) A2 | t = λ t' }.
+Proof.
+  exact (wkTm_red_lam_help w t f eq_refl q).
+Qed.
+
+Proposition wkTm_red_step
+            {B : Type}
+            {F : Type}
+            {ar : F -> ty B}
+            {C1 C2 : con B}
+            {w : wk C1 C2}
+            {A : ty B}
+            {t1 t2 : tm ar C1 A}
+            (p : wWeakened w t1)
+            (r : t1 ~>β t2)
+  : { q : wWeakened w t2 & term_of p ~>β term_of q }.
+Proof.
+  revert p.
+  revert w.
+  revert C2.
+  induction r ; intros C2 w p.
+  - destruct p as [t' p].
+    destruct t' ; simpl in * ; try discriminate.
+    assert (p1 := App_eq_Ty p).
+    assert (p2 := App_eq_fst p).
+    assert (p3 := App_eq_snd p).
+    dependent destruction p.
+    simpl in *.
+    specialize (IHr _ _ (exist _ t'1 p2)).
+    destruct IHr as [q Hq].
+    destruct q as [v q].
+    unshelve eexists.
+    + unshelve eexists.
+      * refine (v · t'2).
+      * simpl.
+        subst.
+        reflexivity.
+    + simpl.
+      apply App_l.
+      assumption.
+  - destruct p as [t' p].
+    destruct t' ; simpl in * ; try discriminate.
+    assert (p1 := App_eq_Ty p).
+    assert (p2 := App_eq_fst p).
+    assert (p3 := App_eq_snd p).
+    dependent destruction p.
+    simpl in *.
+    specialize (IHr _ _ (exist _ t'2 p3)).
+    destruct IHr as [q Hq].
+    destruct q as [v q].
+    unshelve eexists.
+    + unshelve eexists.
+      * refine (t'1 · v).
+      * simpl.
+        subst.
+        reflexivity.
+    + simpl.
+      apply App_r.
+      assumption.
+  - destruct p as [t' p].
+    destruct (wkTm_red_lam w t' f1 p) as [x e].
+    subst.
+    pose (q' := Lam_eq p).
+    specialize (IHr _ (Keep A1 w) (exist _ _ q')).
+    destruct IHr as [z Hz].
+    destruct z as [z Hz'].
+    unshelve eexists.
+    + unshelve eexists.
+      * refine (λ z).
+      * simpl.
+        rewrite  Hz'.
+        reflexivity.
+    + simpl.
+      apply CLam.
+      assumption.
+  - induction r.
+    simpl in *.
+    destruct p as [t' p].
+    destruct t' ; simpl in * ; try discriminate.
+    assert (p1 := App_eq_Ty p).
+    subst.
+    assert (p2 := App_eq_fst p).
+    assert (p3 := App_eq_snd p).
+    rewrite (UIP (App_eq_Ty p) eq_refl) in p2.
+    rewrite (UIP (App_eq_Ty p) eq_refl) in p3.
+    simpl in *.
+    destruct (wkTm_red_lam w t'1 f p2) as [x' e].
+    subst.
+    simpl in *.
+    unshelve eexists.
+    + unshelve eexists.
+      * exact (subTm x' (beta_sub t'2)).
+      * abstract
+          (rewrite <- (Lam_eq p2) ;
+           rewrite !wkTm_is_subTm ;
+           rewrite !subTm_comp ;
+           f_equal ;
+           simpl ; cbn ;
+           rewrite Sub_id_left ;
+           f_equal ;
+           unfold beta_sub ;
+           simpl ;
+           rewrite dropSub_is_compSubWk ;
+           rewrite <- compSub_compWkSub ;
+           simpl ; cbn; 
+           rewrite compWkSub_id ; 
+           rewrite Sub_id_right ; 
+           reflexivity).
+    + simpl.
+      apply CStep.
+      apply Beta.
+Qed.
+
+Proposition wkTm_red
+            {B : Type}
+            {F : Type}
+            {ar : F -> ty B}
+            {C1 C2 : con B}
+            (w : wk C1 C2)
+            {A : ty B}
+            {t1 t2 : tm ar C1 A}
+            (p : wWeakened w t1)
+            (r : t1 ~>β* t2)
+  : { q : wWeakened w t2 & term_of p ~>β* term_of q }.
+Proof.
+  induction r as [ ? ? r | ? ? ? r1 IHr1 r2 IHr2].
+  - pose (wkTm_red_step p r) as H.
+    destruct H as [q Hq].
+    exists q.
+    apply betaRed_step.
+    exact Hq.
+  - specialize (IHr1 p).
+    destruct IHr1 as [q Hq].
+    specialize (IHr2 q).
+    destruct IHr2 as [q' Hq'].
+    exists q'.
+    exact (beta_Trans Hq Hq').
+Qed.
+
+
+(** ** Beta reduction *)
+Definition BetaRed_Wk
+           {B F : Type}
+           {ar : F -> ty B}
+           {C1 C2 : con B}
+           {A : ty B}
+           {t1 t2 : tm ar C2 A}
+           (w : wk C1 C2)
+           (p : t1 ~>β* t2)
+  : wkTm t1 w ~>β* wkTm t2 w.
+Proof.
+  revert w.
+  revert C1.
+  induction p ; intros C1 w ; simpl.
+  - apply betaRed_step.
+    revert C1 w.    
+    induction r ; intros C1 w.
+    + exact (App_l _ (IHr _ w)).
+    + exact (App_r _ (IHr _ w)).
+    + exact (CLam (IHr _ (Keep A1 w))).
+    + apply CStep.
+      induction r.
+      rewrite !wkTm_is_subTm.
+      rewrite subTm_comp.
+      unfold beta_sub.
+      rewrite <- beta_sub_help.
+      rewrite <- subTm_comp.
+      apply Beta.
+  - exact (beta_Trans (IHp1 C1 w) (IHp2 C1 w)).
+Qed.
+
+(** Rewriting is closed under substitution *)
+Definition BetaRed_sub
+           {B F : Type}
+           {ar : F -> ty B}
+           {C1 C2 : con B}
+           {A : ty B}
+           {t1 t2 : tm ar C2 A}
+           (s : sub ar C1 C2)
+           (p : t1 ~>β* t2)
+  : subTm t1 s ~>β* subTm t2 s.
+Proof.
+  revert s.
+  revert C1.
+  induction p ; intros C1 s ; simpl.
+  - apply betaRed_step.
+    revert C1 s.    
+    induction r ; intros C1 s.
+    + exact (App_l _ (IHr _ s)).
+    + exact (App_r _ (IHr _ s)).
+    + exact (CLam (IHr _ (keepSub A1 s))).
+    + apply CStep.
+      induction r.
+      simpl.
+      pose (Beta (subTm f (keepSub A1 s)) (subTm x s)) as p.
+      unfold beta_sub in *.
+      assert (subTm (subTm f (keepSub A1 s)) (idSub C1 _ && subTm x s)
+              =
+              subTm (subTm f (idSub C _ && x)) s)
+        as H.
+      {
+        rewrite subTm_comp.
+        unfold keepSub.
+        rewrite dropSub_is_compSubWk.
+        simpl ; cbn.
+        rewrite <- compSub_compWkSub.
+        simpl ; cbn.
+        rewrite compWkSub_id.
+        rewrite Sub_id_right.
+        rewrite subTm_comp.
+        simpl ; cbn.
+        rewrite Sub_id_left.
+        reflexivity.
+      }
+      rewrite H in p.
+      exact p.
+  - exact (beta_Trans (IHp1 C1 s) (IHp2 C1 s)).
+Qed.
+
+(** ** Rewriting in an AFS *)
+
+Import AFSNotation.
+
+(** Rewriting is closed under weakening *)
+Definition Rew_Wk
+           {B F R : Type}
+           {X : afs B F R}
+           {C1 C2 : con B}
+           {A : ty B}
+           {t1 t2 : tm X C2 A}
+           (w : wk C1 C2)
+           (p : rew X t1 t2)
+  : rew X (wkTm t1 w) (wkTm t2 w).
+Proof.
+  revert w.
+  revert C1.
+  induction p ; intros C1 w ; simpl.
+  - apply rew_step.
+    revert C1 w.    
+    induction r ; intros C1 w.
+    + exact (App_l _ (IHr _ w)).
+    + exact (App_r _ (IHr _ w)).
+    + exact (CLam (IHr _ (Keep A1 w))).
+    + apply CStep.
+      induction r.
+      * induction b.
+        rewrite !wkTm_is_subTm.
+        rewrite subTm_comp.
+        unfold beta_sub.
+        rewrite <- beta_sub_help.
+        rewrite <- subTm_comp.
+        apply AFSBeta.
+        apply Beta.
+      * rewrite !wkTm_is_subTm.
+        rewrite !subTm_comp.
+        apply AFSRew.
+  - exact (rew_Trans (IHp1 C1 w) (IHp2 C1 w)).
+Qed.
+
+(** Rewriting is closed under substitution *)
+Definition Rew_sub
+           {B F R : Type}
+           {X : afs B F R}
+           {C1 C2 : con B}
+           {A : ty B}
+           {t1 t2 : tm X C2 A}
+           (s : sub _ C1 C2)
+           (p : rew X t1 t2)
+  : rew X (subTm t1 s) (subTm t2 s).
+Proof.
+  revert s.
+  revert C1.
+  induction p ; intros C1 s ; simpl.
+  - apply rew_step.
+    revert C1 s.    
+    induction r ; intros C1 s.
+    + exact (App_l _ (IHr _ s)).
+    + exact (App_r _ (IHr _ s)).
+    + exact (CLam (IHr _ (keepSub A1 s))).
+    + apply CStep.
+      induction r.
+      * induction b.
+        simpl.
+        apply AFSBeta.
+        pose (Beta (subTm f (keepSub A1 s)) (subTm x s)) as p.
+        unfold beta_sub in *.
+        assert (subTm (subTm f (keepSub A1 s)) (idSub C1 (Arity X) && subTm x s)
+                =
+                subTm (subTm f (idSub C (Arity X) && x)) s)
+          as H.
+        {
+          rewrite subTm_comp.
+          unfold keepSub.
+          rewrite dropSub_is_compSubWk.
+          simpl ; cbn.
+          rewrite <- compSub_compWkSub.
+          simpl ; cbn.
+          rewrite compWkSub_id.
+          rewrite Sub_id_right.
+          rewrite subTm_comp.
+          simpl ; cbn.
+          rewrite Sub_id_left.
+          reflexivity.
+        }
+        rewrite H in p.
+        exact p.
+      * rewrite !subTm_comp.
+        apply AFSRew.
+  - exact (rew_Trans (IHp1 C1 s) (IHp2 C1 s)).
+Qed.
